Start refining the insertion queries using the For/Where machinery
The new ConstraintChecksRefinements file proves the
refine_foreign_key_constraint_via_select lemma, which replaces a foreign
key constraint check with a count on a For, thus making it possible to
reuse the Query-related lemmas to implement efficient foreign key
checks.

examples/Bookstore.experimental.v
@@ -1,6 +1,7 @@
 Section BookStoreExamples.
   Require Import QueryStructureNotations.
   Require Import ListImplementation.
+  Require Import ConstraintChecksRefinements.
   Require Import AdditionalLemmas AdditionalMorphisms.
 
   Unset Implicit Arguments.
@@ -166,13 +167,8 @@ Section BookStoreExamples.
     Notation "?[ A ]" := (if A then true else false) (at level 50).
 
     hone method "NumOrders". {
-      unfold BookStoreListImpl_AbsR in H; split_and.
-
-      setoid_rewrite refineEquiv_pick_ex_computes_to_and;
-      setoid_rewrite refineEquiv_pick_pair;
-      setoid_rewrite refineEquiv_pick_eq';
-      simplify with monad laws; cbv beta;
-      simpl.
+      unfold BookStoreListImpl_AbsR in H0; split_and.
+      simplify with monad laws.
 
       (* Step 1: Move to a concrete representation *)
       rewrite refine_List_Query_In by eassumption.
@@ -203,6 +199,7 @@ Section BookStoreExamples.
       setoid_rewrite map_map; simpl.
       
       setoid_rewrite refine_Permutation_Reflexivity.
+      setoid_rewrite refine_Count.
       simplify with monad laws.
 
       (* Step 3: Pass the database, unmodified *)
@@ -219,14 +216,9 @@ Section BookStoreExamples.
     }
 
     hone method "GetTitles". {
-      unfold BookStoreListImpl_AbsR in H; split_and.
-      
-      setoid_rewrite refineEquiv_pick_ex_computes_to_and;
-      setoid_rewrite refineEquiv_pick_pair;
-      setoid_rewrite refineEquiv_pick_eq';
-      simplify with monad laws; cbv beta;
-      simpl.
- 
+      unfold BookStoreListImpl_AbsR in H0; split_and.
+      simplify with monad laws.
+
       rewrite refine_List_Query_In by eassumption.
       setoid_rewrite refine_List_Query_In_Where; instantiate (1 := _).
       rewrite refine_List_For_Query_In_Return_Permutation.
@@ -238,6 +230,7 @@ Section BookStoreExamples.
 
       setoid_rewrite refine_Permutation_Reflexivity.
       simplify with monad laws.
+      simpl.
 
       unfold BookStoreListImpl_AbsR.
       rewrite refine_pick_val by eauto. 
@@ -246,30 +239,14 @@ Section BookStoreExamples.
     }
 
     hone method "PlaceOrder". {
-      Lemma refine_trivial_if_then_else :
-        forall x,
-          refine 
-            (If_Then_Else x (ret true) (ret false))
-            (ret x).
-      Proof.
-        destruct x; reflexivity.
-      Qed.
-
       Notation " A ! B " := (A ``(B)) (at level 2).
       setoid_rewrite refine_trivial_if_then_else.
 
-
-      unfold BookStoreListImpl_AbsR in H; split_and.
-      
-      setoid_rewrite refineEquiv_pick_ex_computes_to_and;
-      setoid_rewrite refineEquiv_pick_pair;
-      setoid_rewrite refineEquiv_pick_eq';
-      simplify with monad laws; cbv beta;
-      simpl.
+      unfold BookStoreListImpl_AbsR in H0; split_and.
+      simplify with monad laws.
 
       rewrite refine_pick_val by eauto using EnsembleIndexedListEquivalence_pick_new_index.
       simplify with monad laws.
-
 
       Check refine_List_Query_In.
       
@@ -299,186 +276,21 @@ Section BookStoreExamples.
         intros b **; unfold decides; destruct b; intuition.
       Qed.
 
-      Require Import Compare_dec.
+      Require Import List.
 
-      Definition gtb x y :=
-        andb (leb y x) (negb (beq_nat x y)). 
-  
+      
+      Transparent Query_For Count.
 
-        Lemma blah :
-          forall {schm tbl} P,
-          forall (c : UnConstrQueryStructure schm),
-            refine
-              (Pick (fun (b : bool) =>
-               decides b
-                       (exists tup2: @IndexedTuple _,
-                          (GetUnConstrRelation c tbl tup2 /\ P (indexedTuple tup2)))))
-              (Bind 
-                 (Count (For (UnConstrQuery_In c tbl (fun tup => Where (P tup) Return 1))))
-                 (fun count => ret (gtb count 0))).
-        Proof.
-          Transparent Query_For.
+      Print boxed_option.
+      Require Import AdditionalPermutationLemmas.
 
-          unfold refine, decides, Count, Query_In, UnConstrQuery_In,  Query_Where, Query_Return; 
-          unfold Query_For, QueryResultComp, flatten_CompList; intros.
-          inversion_by computes_to_inv; subst.
-          constructor.
- 
-          generalize (GetUnConstrRelation c tbl) H0.
-          clear H0.
-          induction x2.
+      SearchAbout DecideableEnsemble.
+      Opaque Query_For .
+      Opaque Count.
 
-          admit.
+      setoid_rewrite (refine_foreign_key_constraint_via_select (fun (b: Book) => n!sISBN = b!sISBN)); eauto.
 
-          intros.
-          unfold EnsembleListEquivalence in H0.
-
-
-          Lemma snif :
-            forall {heading} P seq ens,
-              computes_to (For (QueryResultComp (heading := heading) ens (fun tup => Where (P tup) Return tup))) seq ->
-              forall x, 
-                List.In x seq -> P x.
-          Proof.
-            unfold refine, decides, Count, Query_In, UnConstrQuery_In,  Query_Where, Query_Return; 
-            unfold Query_For, QueryResultComp; induction seq as [ | head seq' IH ]; intros.
-            
-            intuition.
-
-            inversion_by computes_to_inv.
-
-            Require Import AdditionalPermutationLemmas.
-
-            pose proof (permutation_cons_in H2) as in_x0.
-            apply in_split in in_x0.
-            destruct in_x0 as [ x0_before [ x0_after ? ] ]; subst. 
-            symmetry in H2. apply Permutation_cons_app_inv in H2.
-
-            rewrite map_map in H3.
-
-
-            Definition boxed_option {heading} (P: _ -> Prop) (x: @IndexedTuple heading) :=
-              Pick (fun l : list Tuple => (P x -> ret [indexedTuple x] ↝ l) /\ (~ P x -> l = [])).
-
-            Require Import List.
-            Lemma temp :
-              forall {heading} P x1 x0_before (head: @Tuple heading) x0_after,
-                flatten_CompList 
-                  (map (boxed_option P) x1) ↝ (x0_before ++ head :: x0_after) ->
-                exists x1_before head' x1_after,
-                  x1 = x1_before ++ head' :: x1_after /\
-                  flatten_CompList (map (boxed_option P) x1_before) ↝ x0_before /\
-                  flatten_CompList (map (boxed_option P) [head']  ) ↝ [head]    /\
-                  flatten_CompList (map (boxed_option P) x1_after ) ↝ x0_after.
-            Proof.
-            Admitted.
-
-            Show.
-            assert ( flatten_CompList
-                       (map (boxed_option P) x1)
-                       ↝ x0_before ++ head :: x0_after) as H3' by (clear; admit); clear H3.
-            destruct (temp _ _ _ _ _ H3') as [ x1_before [ head' [ x1_after (_eq & before & middle & after) ] ] ]; subst.
-
-
-            unfold boxed_option in middle; simpl in middle. 
-            Unset Ltac Debug.
-            apply computes_to_inv in middle.
-            destruct middle as [head'' (middle1 & middle2)].
-            apply computes_to_inv in middle1.
-            apply computes_to_inv in middle2.
-            destruct middle1 as ( spec1 & spec2 ).
-            destruct middle2 as [ nil' (ret_nil & ret_cons) ].
-            (* inversion_by computes_to_inv. (* broken *) *)
-
-            apply computes_to_inv in ret_nil; subst.
-            rewrite app_nil_r in *; subst.
-            apply computes_to_inv in ret_cons; subst.
-
-            Lemma singleton_neq_nil :
-              forall {A} (a: A),
-                [a] = [] <-> False.
-            Proof.
-              intuition discriminate.
-            Qed.              
-
-            rewrite singleton_neq_nil in spec2.
-            assert (forall a, ~ ~ P a -> P a) as excl by (clear; admit).
-            apply excl in spec2.
-            specialize (spec1 spec2).
-
-            apply computes_to_inv in spec1.
-            injection spec1; intros; subst.
-
-            destruct H0.
-
-            subst x; intuition. (* deduce from H3 *)
-            
-            eapply IH; eauto.
-            
-            econstructor; [ | constructor; symmetry; eassumption ].
-            econstructor.
-
-            constructor.
-            instantiate (1 := x1_before ++ x1_after).
-            instantiate (1 := fun x => ens x /\ x <> head').
-
-            admit. (*use non-duplication*)
-
-            (* TODO: Montrer que head est dans x1, découper x1, découper ens *)
-            
-            Lemma flatten_CompList_app :
-              forall {A} x1 x2 x1' x2',
-                flatten_CompList x1 ↝ x1' ->
-                flatten_CompList x2 ↝ x2' ->
-                @flatten_CompList A (x1 ++ x2) ↝ (x1' ++ x2').
-            Proof.
-              induction x1; simpl; intros.
-              inversion_by computes_to_inv; subst.
-
-              rewrite !app_nil_l; assumption.
-              inversion_by computes_to_inv.
-
-              specialize (IHx1 x2 x0 x2' H2 H0). 
-              econstructor; eauto.
-              econstructor; eauto.
-              subst; rewrite app_assoc; constructor.
-            Qed.
-
-            rewrite !map_app.
-            apply flatten_CompList_app.
-
-
-                                 
-                                 flatten_CompList
-  (map
-        (fun tup : Tuple =>
-           {l : list Tuple | P tup -> ret [tup] ↝ l /\ ~ P tup -> l = []})
-        (map indexedTuple (x1_before ++ x1_after))) ↝ 
-     x0_before ++ x0_after
-            econstructor; try eassumption.
-            
-            destruct H0; subst.
-            generalize x1, (GetUnConstrRelation c tbl), H1, H3.
-            clear H1 H3 x1.
-
-            induction x1 as [ | head_x1 x1' IHx1 ];
-              simpl in *;
-              intros;
-              inversion_by computes_to_inv;
-              subst.
-            
-            apply Permutation_length in H2; simpl in H2; discriminate.
-            
-            destruct inversion_by computes_to_inv.
-            simpl in H.
-            
-          
-        Admitted.
-
-        Show.
-        setoid_rewrite (blah (fun (b: Book) => n!sISBN = b!sISBN)).
-
-      simplify with monad laws.
+      simplify with monad laws; simpl.
       
       rewrite refine_List_Query_In by eassumption.
       setoid_rewrite refine_List_Query_In_Where; instantiate (1 := _).
@@ -488,6 +300,7 @@ Section BookStoreExamples.
               (@None string, (Some n!sISBN, @nil (TSearchTermMatcher BookSchema))).
 
       setoid_rewrite (bfind_correct _).
+      setoid_rewrite refine_Count.
       setoid_rewrite refine_Permutation_Reflexivity.
       simplify with monad laws.
 
@@ -495,22 +308,6 @@ Section BookStoreExamples.
       unfold BookStoreListImpl_AbsR.
       
       Split Constraint Checks.
-
-      
-      set (aa := fun a:TBookStorage => EnsembleIndexedListEquivalence
-              ((UpdateUnConstrRelation c ``(sORDERS)
-                  (EnsembleInsert
-                     {|
-                     tupleIndex := Datatypes.length (benumerate (Bag := BagProof OrderStorage) (snd r_n));
-                     indexedTuple := n |} c!sORDERS))!sBOOKS)%QueryImpl
-              (benumerate (Bag := BagProof BookStorage) a)).
-      set (bb := fun a: TOrderStorage => EnsembleIndexedListEquivalence
-              ((UpdateUnConstrRelation c ``(sORDERS)
-                  (EnsembleInsert
-                     {|
-                     tupleIndex := Datatypes.length (benumerate (Bag := BagProof OrderStorage)  (snd r_n));
-                     indexedTuple := n |} c!sORDERS))!sORDERS)%QueryImpl
-              (benumerate (Bag := BagProof OrderStorage) a)).
 
       Definition ID {A}  := fun (x: A) => x.
 
@@ -527,25 +324,6 @@ Section BookStoreExamples.
       setoid_rewrite refineEquiv_pick_pair.
       unfold ID; simpl.
       simplify with monad laws.
-      
-      (*
-      pose proof (refineEquiv_pick_pair (fun a:TBookStorage => EnsembleIndexedListEquivalence
-              ((UpdateUnConstrRelation c ``(sORDERS)
-                  (EnsembleInsert
-                     {|
-                     tupleIndex := Datatypes.length (benumerate (Bag := BagProof OrderStorage) (snd r_n));
-                     indexedTuple := n |} c!sORDERS))!sBOOKS)%QueryImpl
-              (benumerate (Bag := BagProof BookStorage) a)) (fun a: TOrderStorage => EnsembleIndexedListEquivalence
-              ((UpdateUnConstrRelation c ``(sORDERS)
-                  (EnsembleInsert
-                     {|
-                     tupleIndex := Datatypes.length (benumerate (Bag := BagProof OrderStorage)  (snd r_n));
-                     indexedTuple := n |} c!sORDERS))!sORDERS)%QueryImpl
-              (benumerate (Bag := BagProof OrderStorage) a))).
-
-      setoid_rewrite H3; clear H3.
-      simplify with monad laws.
-      *)
 
       rewrite (refine_pick_val' (fst r_n)) by ((*apply (fun id => @refine_list_insert_in_other_table _ c id _ (benumerate (Bag := BagProof BookStorage) (fst r_n)) H1);*) 
                                                intuition discriminate).
@@ -553,18 +331,10 @@ Section BookStoreExamples.
 
       rewrite refine_pick_val by (apply (binsert_correct_DB (store_is_bag := BagProof OrderStorage) _ _ _ _ H2); eauto).
       simplify with monad laws.
-
       reflexivity.
 
       rewrite refine_pick_val by eauto.
-      
       reflexivity.
-      
-      Transparent Query_For.
-
-      clear.
-      generalize_all.
-
 
 
       constructor.
