src/QueryStructure/Refinements/AdditionalFlatMapLemmas.v
@@ -1,0 +1,13 @@
+Require Import List Permutation AdditionalLemmas AdditionalMorphisms Program Arith Morphisms.
+(* TODO: Actually use this file *)
+
+Lemma length_flat_map :
+  forall {A B} seq (f: A -> list B),
+    List.length (flat_map f seq) = 
+    fold_left (fun count (x : A) => count + List.length (f x)) seq 0.
+Proof.
+  intros; 
+  rewrite (Permutation_length (flat_map_rev_permutation seq f));
+  rewrite flat_map_flatten, length_flatten, <- foldright_compose, fold_left_rev_right;
+  unfold compose; simpl; setoid_rewrite plus_comm at 1.
+Qed.
