src/QueryStructure/Refinements/ConstraintChecksRefinements.v
@@ -1,0 +1,149 @@
+Require Export QueryStructureNotations QueryQSSpecs ListImplementation.
+Require Import List Compare_dec AdditionalLemmas AdditionalPermutationLemmas AdditionalMorphisms EnsembleListEquivalenceProperties flattenCompListProperties.
+
+Unset Implicit Arguments.
+
+Definition gtb x y :=
+  andb (leb y x) (negb (beq_nat x y)). 
+
+Transparent Count Query_For.
+
+Lemma For_computes_to_In :
+  forall {heading} P,
+    (forall a, P a \/ ~ P a) ->
+    forall seq ens,
+      computes_to (For (QueryResultComp (heading := heading) ens 
+                                        (fun tup => Where (P tup) Return tup))) seq ->
+      forall x, 
+        List.In x seq -> (P x /\ (exists x0, ens x0 /\ indexedTuple x0 = x)).
+Proof.
+  unfold refine, decides, Count, Query_In, UnConstrQuery_In,  Query_Where, Query_Return; 
+  unfold Query_For, QueryResultComp; intros * excl;
+  induction seq as [ | head seq' IH ]; intros.
+  
+  exfalso; intuition.
+  
+  inversion_by computes_to_inv.
+  
+  pose proof (permutation_cons_in H4) as in_x0.
+  apply in_split in in_x0.
+  destruct in_x0 as [ x0_before [ x0_after ? ] ]; subst. 
+  symmetry in H4. apply Permutation_cons_app_inv in H4.
+
+  rewrite map_map in H5.
+  destruct (flatten_CompList_app_cons_inv _ excl _ _ _ _ H5) as [ x1_before [ x1_middle [ head' [ x1_after (_eq & in_orig & before & middle & after) ] ] ] ]; subst.
+  
+  unfold boxed_option in middle; simpl in middle. 
+  apply computes_to_inv in middle.
+  destruct middle as [head'' (middle1 & middle2)].
+  apply computes_to_inv in middle1.
+  apply computes_to_inv in middle2.
+  destruct middle1 as ( spec1 & spec2 ).
+  destruct middle2 as [ nil' (ret_nil & ret_cons) ].
+  apply computes_to_inv in ret_nil; subst.
+  rewrite app_nil_r in *; subst.
+  apply computes_to_inv in ret_cons; subst.
+
+  rewrite singleton_neq_nil in spec2.
+  destruct (excl head') as [ H | H ]; try solve [exfalso; intuition].
+  specialize (spec1 H).
+
+  apply computes_to_inv in spec1.
+  injection spec1; intros; subst.
+
+  destruct H0.
+
+  - subst x; split; [ | exists head'; split; [ apply H3  | ] ]; auto.
+  - pose proof (EnsembleListEquivalence_slice _ _ _ H3) as smaller_equiv.
+    pose proof (flatten_CompList_app _ _ _ _ before after) as flatten_app. 
+    set (smaller_ens := (fun x : IndexedTuple => ens x /\ ~ In x x1_middle)).
+    split.
+
+    + eapply H1; try assumption.
+      econstructor; [ | constructor; symmetry; eassumption ]. 
+      econstructor.
+      constructor. 
+
+      apply smaller_equiv.
+
+      unfold boxed_option in *.
+      rewrite !map_app, !map_map.
+      apply flatten_app. 
+    + assert (exists x0 : IndexedTuple, smaller_ens x0 /\ indexedTuple x0 = x) as temp.
+      apply H2; try eassumption.
+      econstructor; [ | constructor; symmetry; eassumption ]. 
+      econstructor.
+      constructor. 
+
+      eassumption.
+      unfold boxed_option in *.
+      rewrite !map_app, !map_map.
+      apply flatten_app. 
+      
+      destruct temp as [ x0 ( ens_x & _eq ) ]; subst.
+      eexists; split; eauto.
+
+      unfold smaller_ens in ens_x; intuition.
+Qed.
+
+
+Lemma For_computes_to_nil :
+  forall {heading} P,
+  forall ens,
+    computes_to (For (QueryResultComp (heading := heading) ens 
+                                      (fun tup => Where (P tup) Return tup))) [] ->
+    forall x,
+      ens x -> ~ (P (indexedTuple x)).
+Proof.
+  unfold refine, decides, Count, Query_In, UnConstrQuery_In,  Query_Where, Query_Return; 
+  unfold Query_For, QueryResultComp; intros **.
+
+                                            inversion_by computes_to_inv.
+  symmetry in H2; apply Permutation_nil in H2; subst.
+  apply H1 in H0.
+  apply in_split in H0.
+  destruct H0 as [ x1_before [ x1_after _eq ] ]; subst.
+  
+  rewrite map_map in H3.
+  eapply flatten_CompList_nil; unfold boxed_option; eauto; intuition.
+Qed.
+
+Lemma decidable_excl :
+  forall {A : Type} (P : Ensemble A) (P_dec : DecideableEnsemble P),
+    (forall (a: A), P a \/ ~ P a).
+Proof.
+  intros ** a.
+  destruct (dec a) eqn:eqdec;
+    [ rewrite dec_decides_P in eqdec | rewrite Decides_false in eqdec ]; intuition.
+Qed.
+
+Lemma refine_foreign_key_constraint_via_select :
+  forall {schm tbl} P (P_dec : DecideableEnsemble P),
+  forall (c : UnConstrQueryStructure schm),
+    refine
+      (Pick (fun (b : bool) =>
+               decides b
+                       (exists tup2: @IndexedTuple _,
+                          (GetUnConstrRelation c tbl tup2 /\ P (indexedTuple tup2)))))
+      (Bind 
+         (Count (For (UnConstrQuery_In c tbl (fun tup => Where (P tup) Return tup))))
+         (fun count => ret (gtb count 0))).
+Proof.
+  unfold refine, Count, UnConstrQuery_In; intros * excl * pick_comp ** .
+  inversion_by computes_to_inv; subst.
+
+  constructor.
+
+  destruct (Datatypes.length x0) eqn:eq_length;
+    destruct x0 as [ | head tail ]; simpl in *; try discriminate; unfold gtb; simpl.
+
+  pose proof (For_computes_to_nil _ (GetUnConstrRelation c tbl) H0). 
+  rewrite not_exists_forall; intro a; rewrite not_and_implication; intros.
+  apply H; trivial.
+
+  apply For_computes_to_In with (x := head) in H0; try solve [intuition].
+  destruct H0 as ( p & [ x0 ( in_ens & _eq ) ] ); subst.
+  eexists; split; eauto.
+
+  apply decidable_excl; assumption.
+Qed.
