src/QueryStructure/Refinements/flattenCompListProperties.v
@@ -1,0 +1,141 @@
+Require Export QueryStructureNotations QueryQSSpecs.
+Require Import List AdditionalLemmas AdditionalMorphisms.
+
+Unset Implicit Arguments.
+
+Definition boxed_option {heading} (P: _ -> Prop) (x: @IndexedTuple heading) :=
+  Pick (fun l : list Tuple => (P x -> ret [indexedTuple x] ↝ l) /\ (~ P x -> l = [])).
+
+Lemma flatten_CompList_app :
+  forall {A} x1 x2 x1' x2',
+    flatten_CompList x1 ↝ x1' ->
+    flatten_CompList x2 ↝ x2' ->
+    @flatten_CompList A (x1 ++ x2) ↝ (x1' ++ x2').
+Proof.
+  induction x1; simpl; intros.
+  inversion_by computes_to_inv; subst.
+
+  rewrite !app_nil_l; assumption.
+  inversion_by computes_to_inv.
+
+  specialize (IHx1 x2 x0 x2' H2 H0). 
+  econstructor; eauto.
+  econstructor; eauto.
+  subst; rewrite app_assoc; constructor.
+Qed.
+
+Lemma boxed_option_nil :
+  forall {heading} (P: @Tuple heading -> Prop),
+  forall x,
+    boxed_option (fun x : IndexedTuple => P x) x ↝ [] ->
+    (~ P x).
+Proof.
+  unfold boxed_option; simpl; intros.
+  (* broken: inversion_by computes_to_inv. *)
+  apply computes_to_inv in H.
+  rewrite ret_computes_to, singleton_neq_nil in H.
+  intuition.
+Qed.
+
+Lemma flatten_CompList_nil :
+  forall {heading} (P: @Tuple heading -> Prop),
+  forall seq,
+    flatten_CompList (map (boxed_option P) seq) ↝ [] ->
+    forall x, List.In x seq -> (~ P x).
+Proof.
+  induction seq; simpl; intros flatten_comp * in_seq.
+  - exfalso; assumption.
+  - inversion_by computes_to_inv.
+    symmetry in H2; rewrite app_eq_nil_iff in H2; destruct H2; subst.
+    destruct in_seq; subst.
+    + apply boxed_option_nil; assumption.
+    + apply IHseq; assumption.
+Qed.
+
+Lemma flatten_CompList_app_inv :
+  forall {heading} P,
+    (forall a, P a \/ ~ P a) ->
+    forall x1 x0_before x0_after,
+      flatten_CompList 
+        (map (@boxed_option heading P) x1) ↝ (x0_before ++ x0_after) ->
+      exists x1_before x1_after,
+        x1 = x1_before ++ x1_after /\
+        flatten_CompList (map (boxed_option P) x1_before) ↝ x0_before /\
+        flatten_CompList (map (boxed_option P) x1_after ) ↝ x0_after.
+Proof.
+  intros * excl; induction x1; simpl; intros.
+
+  - inversion_by computes_to_inv.
+    rewrite app_eq_nil_iff in H.
+    setoid_rewrite app_eq_nil_iff.
+    eexists; eexists; intuition; subst; intuition constructor.
+  - inversion_by computes_to_inv. (* TODO: unfolding boxed_option here crashes inversion_by *)
+    pose proof H0; unfold boxed_option in H0.
+    apply computes_to_inv in H0; simpl in H0.
+    destruct H0 as (spec1 & spec2).
+    destruct (excl a) as [ Ptrue | Pfalse ];
+      [ specialize (spec1 Ptrue); apply computes_to_inv in spec1
+      | specialize (spec2 Pfalse) ]; subst.
+    + rewrite app_singleton in H2. 
+      destruct x0_before as [ | a' x0_before' ] eqn:eq_before; subst.
+      * rewrite app_nil_l in H2.
+        destruct x0_after as [ | a' x0_after]; try discriminate.
+        injection H2; intros; subst.
+        exists (@nil (@IndexedTuple heading)).
+        eexists; repeat split; eauto; simpl; repeat econstructor; eauto.
+      * rewrite <- app_comm_cons in H2.
+        injection H2; intros; subst.
+        destruct (IHx1 x0_before' x0_after H1) as [ x1_before [ x1_after (_eq & comp1 & comp2) ] ];
+          subst.
+        exists (a :: x1_before); exists x1_after.
+        simpl; repeat split; repeat (first [eassumption | econstructor]).
+    + rewrite app_nil_l in H2; subst.
+      destruct (IHx1 x0_before x0_after H1) as [ x1_before [ x1_after (_eq & comp1 & comp2) ] ];
+        subst.
+      exists (a :: x1_before); exists x1_after.
+      simpl; repeat split; repeat (first [eassumption | econstructor]).
+Qed.
+
+Lemma flatten_CompList_singleton :
+  forall {heading} P,
+  forall middle (head: @Tuple heading),
+    flatten_CompList (map (boxed_option P) middle) ↝ [head] ->
+    exists x,
+      List.In x middle /\
+      flatten_CompList (map (boxed_option P) [x]) ↝ [head].
+Proof.
+  induction middle; unfold flatten_CompList; simpl; intros.
+  - apply ret_computes_to in H; discriminate.
+  - inversion_by computes_to_inv.
+    destruct x.
+    + rewrite app_nil_l in H2; subst.
+      destruct (IHmiddle _ H1) as [ x (x_in & flat_comp) ].
+      eexists; eauto.
+    + rewrite <- app_comm_cons in H2; injection H2; intros.
+      symmetry in H; rewrite app_eq_nil_iff in H; destruct H; subst. 
+      exists a; repeat (econstructor; eauto).
+Qed.
+
+Lemma flatten_CompList_app_cons_inv :
+  forall {heading} P,
+    (forall a, P a \/ ~ P a) ->
+    forall x1 x0_before (head: @Tuple heading) x0_after,
+      flatten_CompList 
+        (map (boxed_option P) x1) ↝ (x0_before ++ head :: x0_after) ->
+      exists x1_before x1_middle head' x1_after,
+        x1 = x1_before ++ x1_middle ++ x1_after /\
+        List.In head' x1 /\
+        flatten_CompList (map (boxed_option P) x1_before) ↝ x0_before /\
+        flatten_CompList (map (boxed_option P) [head']  ) ↝ [head]    /\
+        flatten_CompList (map (boxed_option P) x1_after ) ↝ x0_after.
+Proof.
+  intros.
+  apply flatten_CompList_app_inv in H0; try assumption.
+  destruct H0 as [ x1_before [ x1_after (eq_split & comp1 & comp2) ] ]; subst.
+  rewrite <- app_singleton in comp2; apply flatten_CompList_app_inv in comp2; try assumption.
+  destruct comp2 as [ middle [ x1_after' (eq_split' & comp2 & comp3) ] ]; subst.
+  apply flatten_CompList_singleton in comp2.
+  destruct comp2 as [ head' (in_middle & comp2) ].
+  repeat setoid_rewrite in_app_iff.
+  repeat eexists; repeat split; try eassumption; intuition. 
+Qed.
